changing restart predicate

Weidenbach_Book/CDCL_W_Restart.thy
@@ -38,29 +38,22 @@ text \<open>The condition of the differences of cardinality has to be strict.
   See the proof of well-foundedness.\<close>
 inductive cdcl\<^sub>W_merge_with_restart where
 restart_step:
-  "(cdcl\<^sub>W_merge_stgy^^(card (set_mset (learned_clss T)) - card (set_mset (learned_clss S)))) S T
+  "(cdcl\<^sub>W_stgy^^(card (set_mset (learned_clss T)) - card (set_mset (learned_clss S)))) S T
   \<Longrightarrow> card (set_mset (learned_clss T)) - card (set_mset (learned_clss S)) > f n
   \<Longrightarrow> restart T U \<Longrightarrow> cdcl\<^sub>W_merge_with_restart (S, n) (U, Suc n)" |
-restart_full: "full1 cdcl\<^sub>W_merge_stgy S T \<Longrightarrow> cdcl\<^sub>W_merge_with_restart (S, n) (T, Suc n)"
-
-lemma "cdcl\<^sub>W_merge_with_restart S T \<Longrightarrow> cdcl\<^sub>W_merge_restart\<^sup>*\<^sup>* (fst S) (fst T)"
-  by (induction rule: cdcl\<^sub>W_merge_with_restart.induct)
-  (auto dest!: relpowp_imp_rtranclp cdcl\<^sub>W_merge_stgy_tranclp_cdcl\<^sub>W_merge tranclp_into_rtranclp
-     rtranclp_cdcl\<^sub>W_merge_stgy_rtranclp_cdcl\<^sub>W_merge rtranclp_cdcl\<^sub>W_merge_tranclp_cdcl\<^sub>W_merge_restart
-     fw_r_rf cdcl\<^sub>W_rf.restart
-    simp: full1_def)
+restart_full: "full1 cdcl\<^sub>W_stgy S T \<Longrightarrow> cdcl\<^sub>W_merge_with_restart (S, n) (T, Suc n)"
 
 lemma cdcl\<^sub>W_merge_with_restart_rtranclp_cdcl\<^sub>W:
   "cdcl\<^sub>W_merge_with_restart S T \<Longrightarrow> cdcl\<^sub>W\<^sup>*\<^sup>* (fst S) (fst T)"
   by (induction rule: cdcl\<^sub>W_merge_with_restart.induct)
-  (auto dest!: relpowp_imp_rtranclp rtranclp_cdcl\<^sub>W_merge_stgy_rtranclp_cdcl\<^sub>W cdcl\<^sub>W.rf
+  (auto dest!: relpowp_imp_rtranclp rtranclp_cdcl\<^sub>W_stgy_rtranclp_cdcl\<^sub>W cdcl\<^sub>W.rf
     cdcl\<^sub>W_rf.restart tranclp_into_rtranclp simp: full1_def)
 
 lemma cdcl\<^sub>W_merge_with_restart_increasing_number:
   "cdcl\<^sub>W_merge_with_restart S T \<Longrightarrow> snd T = 1 + snd S"
   by (induction rule: cdcl\<^sub>W_merge_with_restart.induct) auto
 
-lemma "full1 cdcl\<^sub>W_merge_stgy S T \<Longrightarrow> cdcl\<^sub>W_merge_with_restart (S, n) (T, Suc n)"
+lemma "full1 cdcl\<^sub>W_stgy S T \<Longrightarrow> cdcl\<^sub>W_merge_with_restart (S, n) (T, Suc n)"
   using restart_full by blast
 
 lemma cdcl\<^sub>W_all_struct_inv_learned_clss_bound:
@@ -125,12 +118,12 @@ proof (rule ccontr)
   text \<open>The following does not hold anymore with the non-strict version of
     cardinality in the definition.\<close>
   { fix i
-    assume "no_step cdcl\<^sub>W_merge_stgy (fst (g i))"
+    assume "no_step cdcl\<^sub>W_stgy (fst (g i))"
     with g[of i]
     have False
       proof (induction rule: cdcl\<^sub>W_merge_with_restart.induct)
         case (restart_step T S n) note H = this(1) and c = this(2) and n_s = this(4)
-        obtain S' where "cdcl\<^sub>W_merge_stgy S S'"
+        obtain S' where "cdcl\<^sub>W_stgy S S'"
           using H c by (metis gr_implies_not0 relpowp_E2)
         then show False using n_s by auto
       next
@@ -142,12 +135,12 @@ proof (rule ccontr)
     m: "m = card (set_mset (learned_clss T)) - card (set_mset (learned_clss (fst (g k))))" and
     "m > f (snd (g k))" and
     "restart T (fst (g (k+1)))" and
-    cdcl\<^sub>W_merge_stgy: "(cdcl\<^sub>W_merge_stgy ^^ m) (fst (g k)) T"
+    cdcl\<^sub>W_stgy: "(cdcl\<^sub>W_stgy ^^ m) (fst (g k)) T"
     using g[of k] H[of "Suc k"] by (force simp: cdcl\<^sub>W_merge_with_restart.simps full1_def)
-  have "cdcl\<^sub>W_merge_stgy\<^sup>*\<^sup>* (fst (g k)) T"
-    using cdcl\<^sub>W_merge_stgy relpowp_imp_rtranclp by metis
+  have "cdcl\<^sub>W_stgy\<^sup>*\<^sup>* (fst (g k)) T"
+    using cdcl\<^sub>W_stgy relpowp_imp_rtranclp by metis
   then have "cdcl\<^sub>W_all_struct_inv T"
-    using inv[of k]  rtranclp_cdcl\<^sub>W_all_struct_inv_inv rtranclp_cdcl\<^sub>W_merge_stgy_rtranclp_cdcl\<^sub>W
+    using inv[of k]  rtranclp_cdcl\<^sub>W_all_struct_inv_inv rtranclp_cdcl\<^sub>W_stgy_rtranclp_cdcl\<^sub>W
     by blast
   moreover have "card (set_mset (learned_clss T)) - card (set_mset (learned_clss (fst (g k))))
       > card (simple_clss (atms_of_mm (init_clss (fst ?S))))"
@@ -157,7 +150,7 @@ proof (rule ccontr)
       by linarith
   moreover
     have "init_clss (fst (g k)) = init_clss T"
-      using \<open>cdcl\<^sub>W_merge_stgy\<^sup>*\<^sup>* (fst (g k)) T\<close> rtranclp_cdcl\<^sub>W_merge_stgy_rtranclp_cdcl\<^sub>W
+      using \<open>cdcl\<^sub>W_stgy\<^sup>*\<^sup>* (fst (g k)) T\<close> rtranclp_cdcl\<^sub>W_stgy_rtranclp_cdcl\<^sub>W
       rtranclp_cdcl\<^sub>W_init_clss inv unfolding cdcl\<^sub>W_all_struct_inv_def by blast
     then have "init_clss (fst ?S) = init_clss T"
       using init_g[of k] by auto
@@ -176,12 +169,12 @@ lemma cdcl\<^sub>W_merge_with_restart_distinct_mset_clauses:
   using assms(2,1,3,4)
 proof (induction)
   case (restart_full S T)
-  then show ?case using rtranclp_cdcl\<^sub>W_merge_stgy_distinct_mset_clauses[of S T] unfolding full1_def
+  then show ?case using rtranclp_cdcl\<^sub>W_stgy_distinct_mset_clauses[of S T] unfolding full1_def
     by (auto dest: tranclp_into_rtranclp)
 next
   case (restart_step T S n U)
   then have "distinct_mset (clauses T)"
-    using rtranclp_cdcl\<^sub>W_merge_stgy_distinct_mset_clauses[of S T] unfolding full1_def
+    using rtranclp_cdcl\<^sub>W_stgy_distinct_mset_clauses[of S T] unfolding full1_def
     by (auto dest: relpowp_imp_rtranclp)
   then show ?case using \<open>restart T U\<close>  unfolding clauses_def
     by (metis  distinct_mset_union fstI restartE subset_mset.le_iff_add union_assoc)
@@ -264,10 +257,10 @@ proof (rule ccontr)
     m: "m = card (set_mset (learned_clss T)) - card (set_mset (learned_clss (fst (g k))))" and
     "m > f (snd (g k))" and
     "restart T (fst (g (k+1)))" and
-    cdcl\<^sub>W_merge_stgy: "(cdcl\<^sub>W_stgy ^^ m) (fst (g k)) T"
+    cdcl\<^sub>W_stgy: "(cdcl\<^sub>W_stgy ^^ m) (fst (g k)) T"
     using g[of k] H[of "Suc k"] by (force simp: cdcl\<^sub>W_with_restart.simps full1_def)
   have "cdcl\<^sub>W_stgy\<^sup>*\<^sup>* (fst (g k)) T"
-    using cdcl\<^sub>W_merge_stgy relpowp_imp_rtranclp by metis
+    using cdcl\<^sub>W_stgy relpowp_imp_rtranclp by metis
   then have "cdcl\<^sub>W_all_struct_inv T"
     using inv[of k]  rtranclp_cdcl\<^sub>W_all_struct_inv_inv rtranclp_cdcl\<^sub>W_stgy_rtranclp_cdcl\<^sub>W by blast
   moreover have "card (set_mset (learned_clss T)) - card (set_mset (learned_clss (fst (g k))))
